proofs/transform/eliminate_inductive.v
@@ -3386,40 +3386,6 @@ Qed.
 
 (*wf_predsym and wf_predsym is invariant under changes in the
   context as long as the signatures have the same elements*)
-Definition eq_sig (g1 g2: context) : Prop :=
-  (forall x, In x (sig_t g1) <-> In x (sig_t g2)) /\
-  (forall x, In x (sig_f g1) <-> In x (sig_f g2)) /\
-  (forall x, In x (sig_p g1) <-> In x (sig_p g2)).
-
-Lemma eq_sig_refl: forall l, eq_sig l l.
-Proof.
-  intros. unfold eq_sig; split_all; intros; reflexivity.
-Qed.
-
-Lemma eq_sig_cons: forall x l1 l2,
-  eq_sig l1 l2 ->
-  eq_sig (x :: l1) (x :: l2).
-Proof.
-  intros. unfold eq_sig in *. split_all; intros;
-  unfold sig_t, sig_f, sig_p in *; simpl;
-  rewrite !in_app_iff; apply or_iff_compat_l; auto.
-Qed.
-
-Lemma eq_sig_sublist g1 g2:
-  eq_sig g1 g2 <-> sublist_sig g1 g2 /\ sublist_sig g2 g1.
-Proof.
-  unfold eq_sig, sublist_sig. split; intros; 
-  destruct_all; split_all; unfold sublist in *; intros; auto;
-  try (apply H; auto); try (apply H0; auto); try (apply H1; auto);
-  split; intros; auto.
-Qed.
-
-Lemma eq_sig_is_sublist g1 g2:
-  eq_sig g1 g2 ->
-  sublist_sig g1 g2.
-Proof.
-  rewrite eq_sig_sublist; intros [H1 H2]; auto.
-Qed.
 
 (*The new context has the same signature*)
 Lemma gen_new_ctx_gamma_eq_sig gamma:
@@ -3539,14 +3505,6 @@ Proof.
   - destruct a; auto. simpl. simpl in *.
     inversion H8; subst. rewrite H29; auto.
   - destruct a; inversion H18; auto; simpl; auto.
-Qed.
-
-Lemma eq_sig_sym g1 g2:
-  eq_sig g1 g2 ->
-  eq_sig g2 g1.
-Proof.
-  unfold eq_sig. intros; destruct_all; split_all; intros; auto;
-  symmetry; auto.
 Qed.
 
 (*And finally, the new context is valid*)
