proofs/transform/eliminate_algebraic.v
@@ -1,0 +1,121 @@
+
+Require Import Task.
+Require Import Pattern PatternProofs Alpha.
+Set Bullet Behavior "Strict Subproofs".
+
+(*TODO: does this work?*)
+Section Map.
+Variable (fn: term -> term) (pn: formula -> formula).
+
+Definition t_map  (t: term) : term :=
+  match t with
+  | Tlet ta x tb => Tlet (fn ta) x (fn tb)
+  | Tmatch t1 ty ps =>
+    Tmatch (fn t1) ty (map (fun x => (fst x, fn (snd x))) ps)
+  | Teps f x => Teps (pn f) x
+  | Tif f t1 t2 => Tif (pn f) (fn t1) (fn t2)
+  | Tfun f tys tms => Tfun f tys (map fn tms)
+  | Tconst _ => t
+  | Tvar _ => t
+  end.
+Definition f_map (f: formula) : formula :=  
+  match f with
+  | Flet t x f => Flet (fn t) x (pn f)
+  | Fmatch t ty ps => Fmatch (fn t) ty (map (fun x => (fst x, pn (snd x))) ps)
+  | Fif f1 f2 f3 => Fif (pn f1) (pn f2) (pn f3)
+  | Fpred f tys tms => Fpred f tys (map fn tms)
+  | Fnot f => Fnot (pn f)
+  | Feq ty t1 t2 => Feq ty (fn t1) (fn t2)
+  | Fbinop b f1 f2 => Fbinop b (pn f1) (pn f2)
+  | Fquant q v f => Fquant q v (pn f)
+  | Ftrue => Ftrue
+  | Ffalse => Ffalse
+  end.
+
+End Map.
+
+
+(** Compile match patterns *)
+
+Fixpoint rewriteT (t: term) : term :=
+  match t with
+  | Tmatch tm ty ps =>
+    let t1 := rewriteT tm in
+    match (compile_bare_single true t1 ty 
+      (map (fun x => (fst x, rewriteT (snd x))) ps)) with
+    | Some t2 => t2
+    | None => t
+    end
+  | _ => t_map rewriteT rewriteF t
+  end
+with rewriteF (f: formula) : formula :=
+  match f with
+  | Fmatch t ty ps =>
+    let t1 := rewriteT t in
+    match (compile_bare_single false t1 ty 
+      (map (fun x => (fst x, rewriteF (snd x))) ps)) with
+    | Some t2 => t2
+    | None => f
+    end
+  | _ => f_map rewriteT rewriteF f
+  end.
+
+Definition rewriteT' t := rewriteT (a_convert_all_t t nil).
+Definition rewriteF' f := rewriteF (a_convert_all_f f nil).
+
+(*And the transformation*)
+Definition compile_match : trans := trans_map rewriteT' rewriteF'.
+
+(*Proofs*)
+(* 
+(*1. Typing*)
+Lemma rewrite_typed gamma t f:
+  (forall ty (Hty: term_has_type gamma t ty),
+    term_has_type gamma (rewriteT t) ty) /\
+  (forall (Hty: formula_typed gamma f),
+    formula_typed gamma (rewriteF f)).
+Proof.
+  revert t f; apply term_formula_ind; simpl; auto;
+  try solve[intros; inversion Hty; subst; constructor; auto].
+  - (*Tfun*) intros f1 tys tms IH ty Hty.
+    inversion Hty; subst.
+    constructor; auto.
+    + rewrite map_length; auto.
+    + assert (Hlen: length tms = length (map (ty_subst (s_params f1) tys) (s_args f1))).
+      { rewrite map_length; auto. }
+      generalize dependent (map (ty_subst (s_params f1) tys) (s_args f1)).
+      revert IH.
+      clear.
+      induction tms as [| thd ttl IH]; intros Hall [| tyh tyt]; auto;
+      try discriminate; simpl.
+      intros Hall2 Hlen.
+      inversion Hall; subst. inversion Hall2; subst.
+      constructor; auto.
+  - (*Tmatch*)
+    intros tm ty ps IHtm IHps ty1 Hty1.
+    destruct (compile_bare_single _ _ _ _) as [o1|] eqn : Hcompile; auto.
+    (*2nd case cannot occur by typing but we don't prove that yet*)
+    unfold compile_bare_single in Hcompile.
+    eapply compile_bare_typed in Hcompile; eauto.
+    Search compile_bare.
+  - intros; inversion Hty; subst; constructor; auto.
+
+
+(*2: Semantics*)
+
+(*3: Simple patterns*)
+
+
+    
+     t ty:
+  term_has_type gamma t ty ->
+  term_has_type gamma (rewriteT t) ty.
+Proof.
+  unfold rewriteT.
+
+Lemma compile_match_sound: sound_trans compile_match.
+Proof.
+  unfold compile_match.
+  apply trans_map_sound. *)
+
+
